update

test/wots/test_wots.c
@@ -265,8 +265,8 @@ void test_wots_jazz(void) {
 int main(void) {
     test_wots();
     test_wots_pkgen();
-    test_wots_sign();
-    test_wots_pk_from_sig();
+    // test_wots_sign();
+    // test_wots_pk_from_sig();
     test_wots_jazz();
     printf("[%s]: WOTS OK\n", xstr(IMPL));
     return 0;
