proof/correctness/Correctness_Hash.ec
@@ -4,19 +4,20 @@ require import AllCore List RealExp IntDiv.
 from Jasmin require import JModel.
 
 require import XMSS_IMPL_PP XMSS_IMPL.
-require import Properties.
+require import Address Notation Primitives.
 
 require import Array8 Array32.
 
+import NBytes.
 
-lemma thash_f_correctness (out:W8.t Array32.t, pub_seed:W8.t Array32.t, addr:W32.t Array8.t) : 
-    hoare [ Mp(Syscall).__thash_f : 
-            arg = (out, pub_seed, addr) ==> 
-            to_list res.`1 = thash_f addr (to_list pub_seed) witness]. 
+lemma thash_f_correct (_out_ : W8.t Array32.t, _pub_seed_ : W8.t Array32.t, _addr_ : W32.t Array8.t) :
+    equiv [Mp(Syscall).__thash_f ~ Chain.thash :
+      arg{1}=(_out_, _pub_seed_, _addr_) /\ arg{2}=(to_list _out_, _addr_, to_list _pub_seed_) ==>
+       res{2}.`1 = to_list res{1}.`1 /\ res{1}.`2 = res{2}.`2].
 proof.
 proc.
-auto => />.
 admit.
 qed.
 
-(* Axiom about hash96 and F *)
+(* axiom sobre prf keygen *)
+(* axiom sobre prf e F *)
