proof/correctness/XMSS.ec
@@ -1,0 +1,11 @@
+pragma Goals : printall.
+
+require import AllCore List RealExp IntDiv.
+from Jasmin require import JModel JArray.
+
+require import Params Parameters Address Notation Primitives Wots.
+require import XMSS_IMPL XMSS_IMPL_PP.
+
+
+
+(******* exported functions ********)
